Remove hoare triples, add haskell code

Haskell/Main.hs
@@ -1,0 +1,13 @@
+import SortedList (cons, nil, fromList, unique)
+
+main :: IO ()
+main = do
+  -- The sorted list [1, 1, 2, 2]
+  let l = cons 1 $ cons 2 $ cons 1 $ cons 2 nil
+  print l
+  print $ "Unique elements " ++ show (unique l)
+
+  let l = [4, 5, 2, 4, 2]
+  let s = fromList l
+  print s
+  print $ "Unique elements " ++ show (unique s)
