Haskell/SortedList.hs
@@ -1,0 +1,29 @@
+-- SortedList.hs:
+-- The most important piece to hide is the SortedList constructor
+module SortedList (unique', SortedList (), nil, cons, toList, unique, fromList) where
+
+import Data.List
+
+unique' :: [Int] -> [Int]
+unique' [] = []
+unique' (x : xs) = x : unique' (dropWhile (== x) xs)
+
+newtype SortedList
+  = -- The "unsafe" constructor, must not be accessible directly by downstream code
+    SortedList [Int]
+  deriving (Show, Eq)
+
+nil :: SortedList
+nil = SortedList []
+
+cons :: Int -> SortedList -> SortedList
+cons x (SortedList l) = SortedList (insert x l)
+
+toList :: SortedList -> [Int]
+toList (SortedList l) = l
+
+unique :: SortedList -> [Int]
+unique (SortedList l) = unique' l
+
+fromList :: [Int] -> SortedList
+fromList = SortedList . sort
