Haskell/Unique.hs
@@ -1,0 +1,16 @@
+import Data.List
+
+unique :: [Int] -> [Int]
+unique [] = []
+unique (x : xs) = x : unique (dropWhile (== x) xs)
+
+sorted :: [Int] -> Bool
+sorted [] = True
+sorted [x] = True
+sorted (x : y : xs) = x <= y && sorted (y : xs)
+
+unique' :: [Int] -> Maybe [Int]
+unique' [] = Just []
+unique' (x : xs)
+  | sorted (x : xs) = (x :) <$> unique' (dropWhile (== x) xs)
+  | otherwise = Nothing
