SortedList/Imperative.lean
@@ -10,7 +10,7 @@ set_option mvcgen.warning false
 -- Inspiration: <https://markushimmel.de/blog/my-first-verified-imperative-program/>
 
 /-- (Locally) imperative version of the functional `unique` function. -/
-def unique (xs : List Int) : Id (List Int) := do
+def unique (xs : List Int) : List Int := Id.run do
   let mut c : Option Int := none -- previous x in the list
   let mut out := [] -- output of the function
 
@@ -26,13 +26,14 @@ def unique (xs : List Int) : Id (List Int) := do
 #eval unique [1, 1, 2, 2, 3]
 
 /-- Every element in the input is in the output -/
-theorem unique_spec_supset (l : List Int) : ⦃⌜True⌝⦄ unique l ⦃⇓r => l ⊆ r⦄ := by
-  mvcgen [unique]
+theorem unique_spec_supset (l : List Int) : l ⊆ unique l := by
+  generalize h : unique l = r
+  apply Id.by_wp h _
+  mvcgen
   case inv =>
     exact ⇓⟨⟨c, out⟩, xs⟩ =>
-      ⌜ (∀ x, some x = c → x ∈ out) ∧ -- c is always in out
+        (∀ x, some x = c → x ∈ out) ∧ -- c is always in out
         xs.pref ⊆ out -- property holds for out
-      ⌝
 
   all_goals simp_all
   case post.success =>
@@ -42,36 +43,33 @@ theorem unique_spec_supset (l : List Int) : ⦃⌜True⌝⦄ unique l ⦃⇓r =>
 abbrev StrictSorted (xs : List Int) := Pairwise (· < ·) xs
 
 /-- Main lemma: Given a sorted list as input, `unique` returns a strictly sorted list. -/
-theorem unique_spec_strictSorted (l : List Int) :
-    ⦃⌜Sorted l⌝⦄ unique l ⦃⇓r => StrictSorted r⦄ := by
-  mvcgen [unique]
+theorem unique_spec_strictSorted (l : List Int) (hl : Sorted l) : StrictSorted (unique l) := by
+  generalize h : unique l = r
+  apply Id.by_wp h _
+  mvcgen
   case inv =>
     exact ⇓⟨⟨c, out⟩, xs⟩ =>
-      ⌜
         (∀ x ∈ out, x ≤ c) ∧ -- out ≤ c
         (∀ x ∈ xs.suff, c ≤ x) ∧ -- c is always ≤ the rest of the input (i.e. suffix)
         StrictSorted out -- property holds for out
-      ⌝
 
   all_goals simp_all
   case post.success =>
     intros
     assumption
 
-  obtain ⟨h1, ⟨h2, h3⟩, h4⟩ := h
-  generalize b.snd = out at *
-  generalize b.fst = c at *
+  · obtain ⟨hout_le, ⟨hc, hc_le⟩, h_strictSorted⟩ := h
+    generalize b.snd = out at *
+    generalize b.fst = c at *
 
-  have lemma1 (y) (hy : y ∈ out) : y < x := by
-    rcases c with _ | c
-    · specialize h1 y hy
-      contradiction
-    · simp_all
-      grind
+    have lemma1 (y) (hy : y ∈ out) : y < x := by
+      rcases c with _ | c
+      · specialize hout_le y hy
+        contradiction
+      · simp_all
+        grind
 
-  refine ⟨?_, ?_, ?_⟩
-  · grind
-  · have hs : (x :: suff).Sorted := by grind
+    have hs : (x :: suff).Sorted := by grind
     simp [Sorted] at hs
     grind
   · grind
@@ -84,18 +82,12 @@ theorem StrictSorted.nodup (h : StrictSorted xs) : Nodup xs := by grind
 theorem StrictSorted.iff : StrictSorted xs ↔ Sorted xs ∧ Nodup xs := by grind
 
 /-- An example for composing above results -/
-theorem unique_spec_nodup (l : List Int) :
-    ⦃⌜Sorted l⌝⦄ unique l ⦃⇓r => Nodup r⦄ := by
-  intro hl
-  apply SPred.entails.trans (unique_spec_strictSorted l) StrictSorted.nodup hl
+theorem unique_spec_nodup (l : List Int) (hl : Sorted l) : Nodup (unique l) := by
+  apply StrictSorted.nodup
+  exact unique_spec_strictSorted l hl
 
 /-- The key property that `unique` must have: Every element in the input is in the output and the output is strictly increasing (or equivalently, doesn't contain duplicates and is sorted). -/
-theorem unique_spec (l : List Int) :
-    ⦃⌜Sorted l⌝⦄ unique l ⦃⇓r => l ⊆ r ∧ StrictSorted r⦄ := by
-  intro hl
-  apply SPred.Tactic.ProofMode.start_entails
-  apply SPred.and_intro
-  · intro _
-    exact unique_spec_supset l trivial
-  · intro _
-    exact unique_spec_strictSorted l hl
+theorem unique_spec (l : List Int) (hl : Sorted l) : let r := unique l; l ⊆ r ∧ StrictSorted r := by
+  constructor
+  · exact unique_spec_supset l
+  · exact unique_spec_strictSorted l hl
