SortedList/Subsingleton.lean
@@ -1,0 +1,21 @@
+-- Instead of `Prop` we can technically use `Type` in lean because `Prop` is a universe of subsingletons: types which have at most one element.
+-- In these universes all elements (proofs) of the same type (proposition) are definitionally equal.
+-- Lean is not meant to be used this way but it is possible.
+
+def Sorted (xs : List Int) : Type :=
+  if xs.Pairwise (· ≤ ·)
+  then Unit
+  else Empty
+
+noncomputable
+def Sorted.cons (h : Sorted xs) (hx : ∀ a ∈ xs, x ≤ a) : Sorted (x :: xs) := by
+  unfold Sorted at *
+  split at h
+  next h1 =>
+    split
+    · exact h
+    next h2 =>
+      simp at h2
+      simp_all
+  next h1 =>
+    nomatch h
